Clean/Gadgets/BLAKE3/BLAKE3G.lean
@@ -123,10 +123,10 @@ theorem completeness (a b c d : Fin 16) : Completeness (F p) (elaborated a b c d
 
   dsimp only [Assumptions, BLAKE3State.Normalized] at h_assumptions
 
-  dsimp only [main, circuit_norm, Xor32.circuit, Addition32.circuit, Rotation32.circuit, Rotation32.elaborated] at henv ⊢
+  dsimp only [main, circuit_norm, Xor32.circuit, Addition32.circuit, Rotation32.circuit, Rotation32.elaborated] at h_env ⊢
   simp only [circuit_norm, and_imp,
     Addition32.Assumptions, Addition32.Spec, Rotation32.Assumptions, Rotation32.Spec,
-    Xor32.Assumptions, Xor32.Spec, getElem_eval_vector] at henv ⊢
+    Xor32.Assumptions, Xor32.Spec, getElem_eval_vector] at h_env ⊢
 
   -- resolve all chains of assumptions
   simp_all only [implies_true, forall_const, and_true]
